model

SmartContracts/ModellingOfBugs/DeusFinacePriceOracleManipulation/ErrorneousAccounting.dfy
@@ -12,45 +12,78 @@
  * under the License.
  */
 
-include "./NonNativeTypes.dfy"
-include "./Contract.dfy"
-include "./Token.dfy"
+// include "./NonNativeTypes.dfy"
+// include "./Contract.dfy"
+// include "./Token.dfy"
 
-import opened NonNativeTypes
+// import opened NonNativeTypes
 
 // datatype Msg = Msg(sender: Account, value: uint256)
 
 // type Address = Account
-
+class address {
+  var m_address: nat;
+}
 class errorneous
 {
+  var k : nat; //product invariant
+  var m_address: address;
   var amount0Out : nat, reserve0 : nat, reserve1 : nat;
-  var token0 : map<errorneous, nat>, token1 : map<errorneous, nat>;
+  var token0 : map<address, nat>, token1 : map<address, nat>;
 
-  method swap(amount1Out : nat, to : errorneous)
-    requires this in token0 && this in token1
-    requires token1[this] == reserve1
-    requires reserve0 - amount0Out == token0[this] && reserve0 > amount0Out >= 0
-    requires amount0Out > 0 && reserve1 > 0 && reserve0 > 0
+  method swap(amount1Out : nat, to : address)
+    requires this.m_address in token0 && this.m_address in token1
+    requires to in token0 && to in token1
+    requires token1[this.m_address] ==  reserve1
+    requires reserve0 - amount0Out == token0[this.m_address]
+    requires amount0Out == 0 //since we don't understand what this var is, we set it to 0.
+    requires amount1Out <= token1[this.m_address]
+    requires reserve1 > 0 && reserve0 > 0
+    requires reserve0 * reserve1 == k
+    requires amount1Out < reserve1
 
     modifies this
 
     ensures reserve0 * reserve1 >= old(reserve0) * old(reserve1)
   {
-    if(0 < amount1Out < token1[this])
-    {
-      token1 := token1[this := token1[this] - amount1Out];
-      token0 := token0[this := havoc()];
-      var balance0, balance1 := token0[this], token1[this];
-      var amount0in : int := balance0 - (reserve0 - amount0Out);
-      var balance0Adj : nat := balance0 * 10000 - amount0in * 22;
-      if(balance0Adj * balance1 >= reserve0 * reserve1 * 1000)
-      {
-        reserve0, reserve1 := balance0, balance1;
-      }
-    }
+    token1 := transfer(token1, amount1Out, to,  this.m_address);
+    token0 := uniswapCall(to);
+    var balance0, balance1 := token0[this.m_address], token1[this.m_address];
+    var amount0in : int := balance0 - (reserve0 - amount0Out);
+    var balance0Adj : int := balance0 * 10000 - amount0in * 22;
+    if(balance0Adj * balance1 >= reserve0 * reserve1 * 10000)
+    {reserve0, reserve1 := balance0, balance1;}
+  }
+
+  method uniswapCall(to: address) returns (newt : map<address, nat>)
+    requires to in token0 && this.m_address in token0
+    requires this.m_address in token1
+    // requires t[to] >= amount
+    // modifies this
+    ensures to in token0 && this.m_address in token0
+    ensures this.m_address in newt
+    ensures reserve0 == old(reserve0) && reserve1 == old(reserve1)
+  {
+    var h : nat := havoc();
+    assume (token0[to] >= h);
+    newt := transfer(token0, h, this.m_address, to);
+  }
+
+  method transfer(t:map<address, nat> , amount:nat, to:address, from: address) returns (newt : map<address, nat>)
+    requires to in t && from in t
+    requires t[from] >= amount
+    ensures from in newt && to in newt
+    // ensures from != to ==> newt[from] == old(t)[from] - amount 
+  {
+    newt := t[from := t[from] - amount];
+    newt := newt[to := t[to] + amount];
+  }
+  constructor(a: address)
+  {
+    m_address := a;
   }
 }
+
 
 function method {:extern} havoc() : nat
   ensures havoc() > 0
